analysis/Analysis/Section_3_4.lean
@@ -9,7 +9,7 @@ I have attempted to make the translation as faithful a paraphrasing as possible 
 Main constructions and results of this section:
 
 - Images and inverse images of (Mathlib) functions, within the framework of Section 3.1 set theory.  (The Section 3.2 functions are now deprecated and will not be used further.)
-
+- Connection with Mathlib's image `f '' S` and preimage `f ⁻¹' S` notions.
 -/
 
 namespace Chapter3
@@ -34,7 +34,7 @@ theorem SetTheory.Set.mem_image {X Y:Set} (f:X → Y) (S: Set) (y:Object) : y �
 theorem SetTheory.Set.image_eq_specify {X Y:Set} (f:X → Y) (S: Set) : image f S = Y.specify (fun y ↦ ∃ x:X, x.val ∈ S ∧ f x = y) := by sorry
 
 /-- Connection with Mathlib's notion of image.  Note the need to utilize the `Subtype.val` coercion to make everything type consistent. -/
-theorem SetTheory.Set.image_eq_image {X Y:Set} (f:X → Y) (S: Set) (y: Object) : y ∈ image f S ↔ y ∈ Subtype.val '' (f '' {x | x.val ∈ S}) := by sorry
+theorem SetTheory.Set.image_eq_image {X Y:Set} (f:X → Y) (S: Set): (image f S: _root_.Set Object) = Subtype.val '' (f '' {x | x.val ∈ S}) := by sorry
 
 
 /-- Example 3.4.2 -/
@@ -42,9 +42,31 @@ abbrev f_3_4_2 : nat → nat := fun n ↦ (2*n:ℕ)
 
 theorem SetTheory.Set.image_f_3_4_2 : image f_3_4_2 {1,2,3} = {2,4,6} := by sorry
 
+/-- Example 3.4.3 is written using Mathlib's notion of image -/
+example : (fun n:ℤ ↦ n^2) '' {-1,0,1,2} = {0,1,4} := by sorry
 
+theorem SetTheory.Set.mem_image_of_eval {X Y:Set} (f:X → Y) (S: Set) (x:X) : x.val ∈ S → (f x).val ∈ image f S := by sorry
 
+theorem SetTheory.Set.mem_image_of_eval_counter : ∃ (X Y:Set) (f:X → Y) (S: Set) (x:X), ¬ ((f x).val ∈ image f S → x.val ∈ S) := by sorry
 
+/-- Definition 3.4.4 (inverse images).  Again, it is not required that U be a subset of Y. -/
+abbrev SetTheory.Set.preimage {X Y:Set} (f:X → Y) (U: Set) : Set := X.specify (P := fun x ↦ (f x).val ∈ U)
+
+theorem SetTheory.Set.mem_preimage {X Y:Set} (f:X → Y) (U: Set) (x:X) : x.val ∈ preimage f U ↔ (f x).val ∈ U := by
+  rw [specification_axiom']
+
+/-- Connection with Mathlib's notion of preimage. -/
+theorem SetTheory.Set.preimage_eq {X Y:Set} (f:X → Y) (U: Set) : ((preimage f U): _root_.Set Object) = Subtype.val '' (f⁻¹' {y | y.val ∈ U}) := by sorry
+
+/-- Example 3.4.5 -/
+theorem SetTheory.Set.preimage_f_3_4_2 : preimage f_3_4_2 {2,4,6} = {1,2,3} := by sorry
+
+theorem SetTheory.Set.image_preimage_f_3_4_2 : image f_3_4_2 (preimage f_3_4_2 {1,2,3}) ≠ {1,2,3} := by sorry
+
+/-- Example 3.4.6 (using the Mathlib notinon of preimage) -/
+example : (fun n:ℤ ↦ n^2) ⁻¹' {0,1,4} = {-2,-1,0,1,2} := by sorry
+
+example : (fun n:ℤ ↦ n^2) ⁻¹' ((fun n:ℤ ↦ n^2) '' {-1,0,1,2}) ≠ {-1,0,1,2} := by sorry
 
 
 end Chapter3
